[pi] Stage work on pi-calculus

examples/formal-languages/pi-calculus/pi_agentScript.sml
@@ -7,7 +7,9 @@
 
 open HolKernel Parse boolLib bossLib;
 
-open pred_setTheory generic_termsTheory binderLib nomsetTheory nomdatatype;
+open pred_setTheory listTheory;
+
+open generic_termsTheory binderLib nomsetTheory nomdatatype;
 
 val _ = new_theory "pi_agent";
 
@@ -31,7 +33,7 @@ val _ = new_theory "pi_agent";
                 | Res ''name pi            (* nu x. P *)
 
        residual = TauR pi
-                | InputR name ''name pi      (* (Bound) input *)
+                | InputS name ''name pi      (* Input *)
                 | BoundOutput name ''name pi (* Bound output *)
                 | FreeOutput name name pi    (* Free output *)
    End
@@ -44,13 +46,14 @@ val tyname1 = "pi";
 val tyname2 = "residual";
 
 (* "Name" is under GVAR (of type 0); There's an extra "Var" under type 1 *)
-val gvar_rep_t = “:unit”;
-val u_tm = mk_var("u", gvar_rep_t);
+val unit_t = “:unit”;
+val u_tm = mk_var("u", unit_t);
 val vp = “(\n ^u_tm. n = 0)”;
 
-(* other operators (type 1) are under GLAM (of type 1) *)
-val glam_rep_t = “:unit + unit + unit + unit + unit + unit + unit + unit + unit”;
-val d_tm = mk_var("d", glam_rep_t);
+(* other operators (type 1) are under GLAM (of type 1), 9 + 4 units *)
+val rep_t = “:unit + unit + unit + unit + unit + unit + unit + unit + unit +
+              unit + unit + unit + unit”;
+val d_tm = mk_var("d", rep_t);
 val lp =
   “(\n ^d_tm tns uns.
      n = 1 /\ ISL d /\                                        (* 1. nil *)
@@ -90,17 +93,58 @@ val lp =
               ISR (OUTR (OUTR (OUTR (OUTR (OUTR d))))) /\
               ISR (OUTR (OUTR (OUTR (OUTR (OUTR (OUTR d)))))) /\
               ISR (OUTR (OUTR (OUTR (OUTR (OUTR (OUTR (OUTR d))))))) /\
+              ISL (OUTR (OUTR (OUTR (OUTR (OUTR (OUTR (OUTR (OUTR d)))))))) /\
               tns = [1] /\ uns = [] \/
-     n = 2 /\ ISL d /\                                        (* tau residual *)
+     n = 2 /\ ISR d /\ ISR (OUTR d) /\ ISR (OUTR (OUTR d)) /\ (* 1. tau residual *)
+              ISR (OUTR (OUTR (OUTR d))) /\
+              ISR (OUTR (OUTR (OUTR (OUTR d)))) /\
+              ISR (OUTR (OUTR (OUTR (OUTR (OUTR d))))) /\
+              ISR (OUTR (OUTR (OUTR (OUTR (OUTR (OUTR d)))))) /\
+              ISR (OUTR (OUTR (OUTR (OUTR (OUTR (OUTR (OUTR d))))))) /\
+              ISR (OUTR (OUTR (OUTR (OUTR (OUTR (OUTR (OUTR (OUTR d)))))))) /\
+              ISL (OUTR (OUTR (OUTR (OUTR (OUTR (OUTR (OUTR (OUTR (OUTR d))))))))) /\
               tns = [] ∧ uns = [1] \/
-     n = 2 /\ ISR d /\ ISL (OUTR d) /\                        (* bound output *)
+     n = 2 /\ ISR d /\ ISR (OUTR d) /\ ISR (OUTR (OUTR d)) /\ (* 2. bound output *)
+              ISR (OUTR (OUTR (OUTR d))) /\
+              ISR (OUTR (OUTR (OUTR (OUTR d)))) /\
+              ISR (OUTR (OUTR (OUTR (OUTR (OUTR d))))) /\
+              ISR (OUTR (OUTR (OUTR (OUTR (OUTR (OUTR d)))))) /\
+              ISR (OUTR (OUTR (OUTR (OUTR (OUTR (OUTR (OUTR d))))))) /\
+              ISR (OUTR (OUTR (OUTR (OUTR (OUTR (OUTR (OUTR (OUTR d)))))))) /\
+              ISR (OUTR (OUTR (OUTR (OUTR (OUTR (OUTR (OUTR (OUTR (OUTR d))))))))) /\
+              ISL (OUTR (OUTR (OUTR (OUTR (OUTR (OUTR (OUTR (OUTR (OUTR
+                  (OUTR d)))))))))) /\
               tns = [1] /\ uns = [0] \/
-     n = 2 /\ ISR d /\ ISR (OUTR d) /\ ISL (OUTR (OUTR d)) /\ (* input residual *)
+     n = 2 /\ ISR d /\ ISR (OUTR d) /\ ISR (OUTR (OUTR d)) /\ (* 3. input residual *)
+              ISR (OUTR (OUTR (OUTR d))) /\
+              ISR (OUTR (OUTR (OUTR (OUTR d)))) /\
+              ISR (OUTR (OUTR (OUTR (OUTR (OUTR d))))) /\
+              ISR (OUTR (OUTR (OUTR (OUTR (OUTR (OUTR d)))))) /\
+              ISR (OUTR (OUTR (OUTR (OUTR (OUTR (OUTR (OUTR d))))))) /\
+              ISR (OUTR (OUTR (OUTR (OUTR (OUTR (OUTR (OUTR (OUTR d)))))))) /\
+              ISR (OUTR (OUTR (OUTR (OUTR (OUTR (OUTR (OUTR (OUTR (OUTR d))))))))) /\
+              ISR (OUTR (OUTR (OUTR (OUTR (OUTR (OUTR (OUTR (OUTR (OUTR
+                  (OUTR d)))))))))) /\
+              ISL (OUTR (OUTR (OUTR (OUTR (OUTR (OUTR (OUTR (OUTR (OUTR
+                  (OUTR (OUTR d))))))))))) /\
               tns = [1] /\ uns = [0] \/
-     n = 2 /\ ISR d /\ ISR (OUTR d) /\ ISR (OUTR (OUTR d)) /\ (* free output *)
-              ISL (OUTR (OUTR (OUTR d))) /\
+     n = 2 /\ ISR d /\ ISR (OUTR d) /\ ISR (OUTR (OUTR d)) /\ (* 4. free output *)
+              ISR (OUTR (OUTR (OUTR d))) /\
+              ISR (OUTR (OUTR (OUTR (OUTR d)))) /\
+              ISR (OUTR (OUTR (OUTR (OUTR (OUTR d))))) /\
+              ISR (OUTR (OUTR (OUTR (OUTR (OUTR (OUTR d)))))) /\
+              ISR (OUTR (OUTR (OUTR (OUTR (OUTR (OUTR (OUTR d))))))) /\
+              ISR (OUTR (OUTR (OUTR (OUTR (OUTR (OUTR (OUTR (OUTR d)))))))) /\
+              ISR (OUTR (OUTR (OUTR (OUTR (OUTR (OUTR (OUTR (OUTR (OUTR d))))))))) /\
+              ISR (OUTR (OUTR (OUTR (OUTR (OUTR (OUTR (OUTR (OUTR (OUTR
+                  (OUTR d)))))))))) /\
+              ISR (OUTR (OUTR (OUTR (OUTR (OUTR (OUTR (OUTR (OUTR (OUTR
+                  (OUTR (OUTR d))))))))))) /\
               tns = [] /\ uns = [0; 0; 1]
     )”;
+
+(* This is often useful for debugging purposes *)
+Overload LP = lp;
 
 (* type 0 (:name) *)
 val {term_ABS_pseudo11 = term_ABS_pseudo11_0,
@@ -304,7 +348,7 @@ val Res_t = mk_var("Res", “:string -> ^newty1 -> ^newty1”);
 val Res_def = new_definition(
    "Res_def",
   “^Res_t v P =
-   ^term_ABS_t1 (GLAM v (INR (INR (INR (INR (INR (INR (INR (INR ()))))))))
+   ^term_ABS_t1 (GLAM v (INR (INR (INR (INR (INR (INR (INR (INR (INL ())))))))))
                         [^term_REP_t1 P] [])”);
 val Res_tm = Res_def |> concl |> strip_forall |> snd |> rhs |> rand;
 val Res_termP = prove(
@@ -316,14 +360,21 @@ val Res_t = defined_const Res_def;
 val TauR_t = mk_var("TauR", “:^newty1 -> ^newty2”);
 val TauR_def = new_definition(
    "TauR_def",
-  “^TauR_t P = ^term_ABS_t2 (GLAM ARB (INL ()) [] [^term_REP_t1 P])”);
+  “^TauR_t P =
+   ^term_ABS_t2 (GLAM ARB (INR (INR (INR (INR (INR (INR (INR (INR (INR
+                               (INL ()))))))))))
+                          [] [^term_REP_t1 P])”);
 val TauR_tm = TauR_def |> concl |> strip_forall |> snd |> rhs |> rand;
 val TauR_termP = prove(
-   “^termP2 (GLAM x (INL ()) [] [^term_REP_t1 P])”,
+   “^termP2 (GLAM x (INR (INR (INR (INR (INR (INR (INR (INR (INR
+                              (INL ()))))))))))
+                    [] [^term_REP_t1 P])”,
     match_mp_tac glam >> srw_tac [][genind_term_REP1]);
 val TauR_t = defined_const TauR_def;
 val TauR_def' = prove(
-  “^term_ABS_t2 (GLAM v (INL ()) [] [^term_REP_t1 P]) = ^TauR_t P”,
+  “^term_ABS_t2 (GLAM v (INR (INR (INR (INR (INR (INR (INR (INR (INR
+                             (INL ()))))))))))
+                        [] [^term_REP_t1 P]) = ^TauR_t P”,
     srw_tac [][TauR_def, GLAM_NIL_EQ, term_ABS_pseudo11_2, TauR_termP]);
 
 (* Bound output (residual) *)
@@ -331,48 +382,53 @@ val BoundOutput_t =
     mk_var("BoundOutput", “:^newty0 -> string -> ^newty1 -> ^newty2”);
 val BoundOutput_def = new_definition(
    "BoundOutput_def",
-  “^BoundOutput_t a x P = ^term_ABS_t2 (GLAM x (INR (INL ()))
-                                               [^term_REP_t1 P]
-                                               [^term_REP_t0 a])”);
+  “^BoundOutput_t a x P =
+   ^term_ABS_t2 (GLAM x (INR (INR (INR (INR (INR (INR (INR (INR (INR (INR
+                             (INL ())))))))))))
+                        [^term_REP_t1 P] [^term_REP_t0 a])”);
 val BoundOutput_termP = prove(
     mk_comb(termP2, BoundOutput_def |> SPEC_ALL |> concl |> rhs |> rand),
     match_mp_tac glam >> srw_tac [][genind_term_REP0, genind_term_REP1]);
 val BoundOutput_t = defined_const BoundOutput_def;
 
 (* Input residual *)
-val InputR_t = mk_var("InputR",
-                             “:^newty0 -> string -> ^newty1 -> ^newty2”);
-val InputR_def = new_definition(
-   "InputR_def",
-  “^InputR_t a x P = ^term_ABS_t2 (GLAM x (INR (INR (INL ())))
-                                                 [^term_REP_t1 P]
-                                                 [^term_REP_t0 a])”);
-val InputR_termP = prove(
-    mk_comb(termP2, InputR_def |> SPEC_ALL |> concl |> rhs |> rand),
+val InputS_t = mk_var("InputS", “:^newty0 -> string -> ^newty1 -> ^newty2”);
+val InputS_def = new_definition(
+   "InputS_def",
+  “^InputS_t a x P =
+   ^term_ABS_t2 (GLAM x (INR (INR (INR (INR (INR (INR (INR (INR (INR (INR (INR
+                             (INL ()))))))))))))
+                        [^term_REP_t1 P] [^term_REP_t0 a])”);
+val InputS_termP = prove(
+    mk_comb(termP2, InputS_def |> SPEC_ALL |> concl |> rhs |> rand),
     match_mp_tac glam >> srw_tac [][genind_term_REP0, genind_term_REP1]);
-val InputR_t = defined_const InputR_def;
+val InputS_t = defined_const InputS_def;
 
 (* Free output (residual) *)
 val FreeOutput_t =
     mk_var("FreeOutput", “:^newty0 -> ^newty0 -> ^newty1 -> ^newty2”);
 val FreeOutput_def = new_definition(
    "FreeOutput_def",
-  “^FreeOutput_t a b P = ^term_ABS_t2 (GLAM ARB (INR (INR (INR (INL ())))) []
-                                            [^term_REP_t0 a;
-                                             ^term_REP_t0 b;
-                                             ^term_REP_t1 P])”);
+  “^FreeOutput_t a b P =
+   ^term_ABS_t2 (GLAM ARB (INR (INR (INR (INR (INR (INR (INR (INR (INR (INR (INR
+                               (INR ()))))))))))))
+                          [] [^term_REP_t0 a;
+                              ^term_REP_t0 b;
+                              ^term_REP_t1 P])”);
 val FreeOutput_termP = prove(
-   “^termP2 (GLAM x (INR (INR (INR (INL ())))) []
-                                            [^term_REP_t0 a;
-                                             ^term_REP_t0 b;
-                                             ^term_REP_t1 P])”,
+   “^termP2 (GLAM x (INR (INR (INR (INR (INR (INR (INR (INR (INR (INR (INR
+                              (INR ()))))))))))))
+                    [] [^term_REP_t0 a;
+                        ^term_REP_t0 b;
+                        ^term_REP_t1 P])”,
     match_mp_tac glam >> srw_tac [][genind_term_REP0, genind_term_REP1]);
 val FreeOutput_t = defined_const FreeOutput_def;
 val FreeOutput_def' = prove(
-  “^term_ABS_t2 (GLAM v (INR (INR (INR (INL ())))) []
-                                            [^term_REP_t0 a;
-                                             ^term_REP_t0 b;
-                                             ^term_REP_t1 P]) = ^FreeOutput_t a b P”,
+  “^term_ABS_t2 (GLAM v (INR (INR (INR (INR (INR (INR (INR (INR (INR (INR (INR
+                             (INR ()))))))))))))
+                        [] [^term_REP_t0 a;
+                            ^term_REP_t0 b;
+                            ^term_REP_t1 P]) = ^FreeOutput_t a b P”,
     srw_tac [][FreeOutput_def, GLAM_NIL_EQ, term_ABS_pseudo11_2,
                FreeOutput_termP]);
 
@@ -411,7 +467,7 @@ QED
 Theorem npm_CONS :
     npm ((x,y)::pi) (t :name) = npm [(x,y)] (npm pi t)
 Proof
-  SRW_TAC [][GSYM pmact_decompose]
+    SRW_TAC [][GSYM pmact_decompose]
 QED
 
 (* ----------------------------------------------------------------------
@@ -459,7 +515,7 @@ QED
 Theorem tpm_CONS :
     tpm ((x,y)::pi) (t :pi) = tpm [(x,y)] (tpm pi t)
 Proof
-  SRW_TAC [][GSYM pmact_decompose]
+    SRW_TAC [][GSYM pmact_decompose]
 QED
 
 (* ----------------------------------------------------------------------
@@ -469,7 +525,7 @@ QED
 val rcons_info =
     [{con_termP = TauR_termP,        con_def = SYM TauR_def'},
      {con_termP = BoundOutput_termP, con_def = BoundOutput_def},
-     {con_termP = InputR_termP,      con_def = InputR_def},
+     {con_termP = InputS_termP,      con_def = InputS_def},
      {con_termP = FreeOutput_termP,  con_def = SYM FreeOutput_def'}];
 
 val rpm_name_pfx = "r";
@@ -488,8 +544,9 @@ val {tpm_thm = rpm_thm,
                         genind_term_REP = genind_term_REP2};
 
 Theorem rpm_thm[allow_rebind] =
-        rpm_thm |> REWRITE_RULE [GSYM term_REP_npm, GSYM term_REP_tpm, TauR_def',
-                                 GSYM BoundOutput_def, GSYM InputR_def, FreeOutput_def']
+        rpm_thm
+     |> REWRITE_RULE [GSYM term_REP_npm, GSYM term_REP_tpm, TauR_def',
+                      GSYM BoundOutput_def, GSYM InputS_def, FreeOutput_def']
 
 Theorem rpm_eqr :
     t = rpm pi u <=> rpm (REVERSE pi) t = (u :residual)
@@ -506,7 +563,7 @@ QED
 Theorem rpm_CONS :
     rpm ((x,y)::pi) (t :residual) = rpm [(x,y)] (rpm pi t)
 Proof
-  SRW_TAC [][GSYM pmact_decompose]
+    SRW_TAC [][GSYM pmact_decompose]
 QED
 
 (* ----------------------------------------------------------------------
@@ -545,6 +602,8 @@ val supp_npm = prove(
  >> srw_tac [][supp_npm_support, supp_npm_apart, FINITE_GFV]);
 
 val _ = overload_on ("FV", “supp ^n_pmact_t”);
+
+val _ = set_fixity "#" (Infix(NONASSOC, 450));
 val _ = overload_on ("#", “\v (P :name). v NOTIN FV P”);
 
 Theorem FINITE_FV_name[simp] :
@@ -611,8 +670,6 @@ val supp_tpm = prove(
  >> srw_tac [][supp_tpm_support, supp_tpm_apart, FINITE_GFV]);
 
 val _ = overload_on ("FV", “supp ^t_pmact_t”);
-
-val _ = set_fixity "#" (Infix(NONASSOC, 450));
 val _ = overload_on ("#", “\v (P :pi). v NOTIN FV P”);
 
 Theorem FINITE_FV[simp] :
@@ -727,7 +784,7 @@ val LIST_REL_NIL = listTheory.LIST_REL_NIL;
 
 val term_ind =
     bvc_genind
-        |> INST_TYPE [alpha |-> glam_rep_t, beta |-> gvar_rep_t]
+        |> INST_TYPE [alpha |-> rep_t, beta |-> unit_t]
         |> Q.INST [‘vp’ |-> ‘^vp’, ‘lp’ |-> ‘^lp’]
         |> SIMP_RULE std_ss [LIST_REL_CONS1, RIGHT_AND_OVER_OR,
                              LEFT_AND_OVER_OR, DISJ_IMP_THM, LIST_REL_NIL]
@@ -826,5 +883,254 @@ Proof
     SRW_TAC [boolSimps.CONJ_ss][Input_eq_thm, pmact_flip_args]
 QED
 
+(* |- !a b x y t1 t2.
+        InputS a x t1 = InputS b y t2 <=>
+        x = y /\ t1 = t2 /\ a = b \/
+        x <> y /\ x # t2 /\ t1 = tpm [(x,y)] t2 /\ a = b
+ *)
+Theorem InputS_eq_thm =
+  “InputS a x t1 = InputS b y (t2 :pi)”
+     |> SIMP_CONV (srw_ss()) [InputS_def, InputS_termP, term_ABS_pseudo11_2,
+                              GLAM_eq_thm,
+                              term_REP_11_0, term_REP_11_1, term_REP_11_2,
+                              GSYM term_REP_tpm, GSYM term_REP_rpm,
+                              GSYM supp_tpm, GSYM supp_rpm]
+     |> Q.GENL [‘a’, ‘b’, ‘x’, ‘y’, ‘t1’, ‘t2’]
+
+Theorem InputS_tpm_ALPHA :
+    v # (u :pi) ==> InputS a x u = InputS a v (tpm [(v,x)] u)
+Proof
+    SRW_TAC [boolSimps.CONJ_ss][InputS_eq_thm, pmact_flip_args]
+QED
+
+(* ----------------------------------------------------------------------
+    term recursion
+   ---------------------------------------------------------------------- *)
+
+(* NOTE: all 3 types have the same repty *)
+val (_, repty) = dom_rng (type_of term_REP_t0);
+val repty' = ty_antiq repty;
+
+val termP_elim0 = prove(
+   “(!g. ^termP0 g ==> P g) <=> (!t. P (^term_REP_t0 t))”,
+    srw_tac [][EQ_IMP_THM] >- srw_tac [][genind_term_REP0]
+ >> first_x_assum (qspec_then ‘^term_ABS_t0 g’ mp_tac)
+ >> srw_tac [][repabs_pseudo_id0]);
+
+val termP_removal0 =
+    nomdatatype.termP_removal {
+      elimth = termP_elim0, absrep_id = absrep_id0,
+      tpm_def = AP_TERM term_ABS_t0 term_REP_npm |> REWRITE_RULE [absrep_id0],
+      termP = termP0, repty = repty};
+
+val termP_elim1 = prove(
+   “(!g. ^termP1 g ==> P g) <=> (!t. P (^term_REP_t1 t))”,
+    srw_tac [][EQ_IMP_THM] >- srw_tac [][genind_term_REP1]
+ >> first_x_assum (qspec_then ‘^term_ABS_t1 g’ mp_tac)
+ >> srw_tac [][repabs_pseudo_id1]);
+
+val termP_removal1 =
+    nomdatatype.termP_removal {
+      elimth = termP_elim1, absrep_id = absrep_id1,
+      tpm_def = AP_TERM term_ABS_t1 term_REP_tpm |> REWRITE_RULE [absrep_id1],
+      termP = termP1, repty = repty};
+
+val termP_elim2 = prove(
+   “(!g. ^termP2 g ==> P g) <=> (!t. P (^term_REP_t2 t))”,
+    srw_tac [][EQ_IMP_THM] >- srw_tac [][genind_term_REP2]
+ >> first_x_assum (qspec_then ‘^term_ABS_t2 g’ mp_tac)
+ >> srw_tac [][repabs_pseudo_id2]);
+
+val termP_removal2 =
+    nomdatatype.termP_removal {
+      elimth = termP_elim2, absrep_id = absrep_id2,
+      tpm_def = AP_TERM term_ABS_t2 term_REP_rpm |> REWRITE_RULE [absrep_id2],
+      termP = termP2, repty = repty};
+
+val termP' = prove(
+   “genind ^vp ^lp n t <=>
+      ^termP0 t /\ n = 0 \/
+      ^termP1 t /\ n = 1 \/
+      ^termP2 t /\ n = 2”,
+    EQ_TAC >> simp_tac (srw_ss()) [] >> strip_tac >> rw []
+ >> qsuff_tac ‘n = 0 \/ n = 1 \/ n = 2’ >- (strip_tac >> srw_tac [][])
+ >> pop_assum mp_tac
+ >> Q.ISPEC_THEN ‘t’ STRUCT_CASES_TAC gterm_cases
+ >> srw_tac [][genind_GVAR, genind_GLAM_eqn]);
+
+(* “tvf :string -> 'q -> 'r” *)
+val tvf = “λ(s :string) (u :unit) (p :'q). tvf s p :'r”; (* Name *)
+
+(* Type of constants (all constructors are included) occurring in tlf:
+
+   Nil:    “tnf :('q -> 'r)”
+   Tau:    “ttf :('q -> 'r) -> pi -> ('q -> 'r)”
+   Input:  “tif :('q -> 'r) -> string -> ('q -> 'r) ->
+                 name -> pi -> ('q -> 'r)”
+   Output: “tof :('q -> 'r) -> ('q -> 'r) -> ('q -> 'r) ->
+                 name -> name -> pi -> ('q -> 'r)”
+   Match:  “tmf :('q -> 'r) -> ('q -> 'r) -> ('q -> 'r) ->
+                 name -> name -> pi -> ('q -> 'r)”
+   Mismatch: “tuf :('q -> 'r) -> ('q -> 'r) -> ('q -> 'r) ->
+                   name -> name -> pi -> ('q -> 'r)”
+   Sum:    “tsf :('q -> 'r) -> ('q -> 'r) -> pi -> pi -> ('q -> 'r)”
+   Par:    “tpf :('q -> 'r) -> ('q -> 'r) -> pi -> pi -> ('q -> 'r)”
+   Res:    “tcf :string -> ('q -> 'r) -> pi -> ('q -> 'r)”
+
+   TauR:        “taf :('q -> 'r) -> pi -> ('q -> 'r)”
+   InputS:      “trf :('q -> 'r) -> string -> ('q -> 'r) ->
+                      name -> pi -> ('q -> 'r)”
+   BoundOutput: “tbf :('q -> 'r) -> string -> ('q -> 'r) ->
+                      name -> pi -> ('q -> 'r)”
+   FreeOutput:  “tff :('q -> 'r) -> ('q -> 'r) -> ('q -> 'r) ->
+                      name -> name -> pi -> ('q -> 'r)”
+
+   NOTE: ds1 is the list of (bounded) recursive parameters as functions ('q -> 'r).
+         ts1 is the list of (bounded) actual arguments in the same position.
+         ds2 is the list of (unbounded) recursive parameters as functions ('q -> 'r).
+         ts2 is the list of (unbounded) actual arguments in the same position.
+         non-recursive parameters are taken from the corresponding position of u.
+        "if conditions" identify the constructor.
+         v is the only binding variable.
+ *)
+val u_tm = mk_var("u", rep_t);
+
+(* tlf's ty :string ->
+             'a ->
+             ('q -> 'c) list ->
+             ('q -> 'c) list ->
+             ('a, 'b) gterm list -> ('a, 'b) gterm list -> 'q -> 'c)
+ *)
+val tlf =
+   “λ(v :string) ^u_tm (ds1 :('q -> 'r) list) (ds2 :('q -> 'r) list)
+                       (ts1 :^repty' list) (ts2 :^repty' list) (p :'q).
+       if ISL u then                                   (* Nil *)
+         tnf p :'r
+       else if ISL (OUTR u) then                       (* Tau *)
+         ttf (HD ds2) (^term_ABS_t1 (HD ts2)) p :'r
+       else if ISL (OUTR (OUTR u)) then                (* Input *)
+         tif (HD ds2) v (HD ds1)
+             (^term_ABS_t0 (HD ts2)) (^term_ABS_t1 (HD ts1)) p :'r
+       else if ISL (OUTR (OUTR (OUTR u))) then         (* Output *)
+         tof (HD ds2) (HD (TL ds2)) (HD (TL (TL ds2)))
+             (^term_ABS_t0 (HD ts2))
+             (^term_ABS_t0 (HD (TL ts2)))
+             (^term_ABS_t1 (HD (TL (TL ts2)))) p :'r
+       else if ISL (OUTR (OUTR (OUTR (OUTR u)))) then  (* Match *)
+         tmf (HD ds2) (HD (TL ds2)) (HD (TL (TL ds2)))
+             (^term_ABS_t0 (HD ts2))
+             (^term_ABS_t0 (HD (TL ts2)))
+             (^term_ABS_t1 (HD (TL (TL ts2)))) p :'r
+       else if ISL (OUTR (OUTR (OUTR (OUTR (OUTR u))))) then (* Mismatch *)
+         tuf (HD ds2) (HD (TL ds2)) (HD (TL (TL ds2)))
+             (^term_ABS_t0 (HD ts2))
+             (^term_ABS_t0 (HD (TL ts2)))
+             (^term_ABS_t1 (HD (TL (TL ts2)))) p :'r
+       else if ISL (OUTR (OUTR (OUTR (OUTR (OUTR (OUTR u)))))) then (* Sum *)
+         tsf (HD ds2) (HD (TL ds2))
+             (^term_ABS_t1 (HD ts2))
+             (^term_ABS_t1 (HD (TL ts2))) p :'r
+       else if ISL (OUTR (OUTR (OUTR (OUTR (OUTR (OUTR (OUTR u))))))) then (* Par *)
+         tpf (HD ds2) (HD (TL ds2))
+             (^term_ABS_t1 (HD ts2))
+             (^term_ABS_t1 (HD (TL ts2))) p :'r
+       else if ISL (OUTR (OUTR (OUTR (OUTR (OUTR (OUTR (OUTR (* Res *)
+                   (OUTR u)))))))) then
+         tcf v (HD ds1) (^term_ABS_t1 (HD ts1)) p :'r
+       else if ISL (OUTR (OUTR (OUTR (OUTR (OUTR (OUTR (OUTR (* TauR *)
+                   (OUTR (OUTR u))))))))) then
+         taf (HD ds2) (^term_ABS_t1 (HD ts2)) p :'r
+       else if ISL (OUTR (OUTR (OUTR (OUTR (OUTR (OUTR (OUTR (* InputS *)
+                   (OUTR (OUTR (OUTR u)))))))))) then
+         trf (HD ds2) v (HD ds1)
+             (^term_ABS_t0 (HD ts2)) (^term_ABS_t1 (HD ts1)) p :'r
+       else if ISL (OUTR (OUTR (OUTR (OUTR (OUTR (OUTR (OUTR (* BoundOutput *)
+                   (OUTR (OUTR (OUTR (OUTR u))))))))))) then
+         tbf (HD ds2) v (HD ds1)
+             (^term_ABS_t0 (HD ts2)) (^term_ABS_t1 (HD ts1)) p :'r
+       else
+         tof (HD ds2) (HD (TL ds2)) (HD (TL (TL ds2)))
+             (^term_ABS_t0 (HD ts2))
+             (^term_ABS_t0 (HD (TL ts2)))
+             (^term_ABS_t1 (HD (TL (TL ts2)))) p :'r”;
+
+Overload TLF = tlf
+
+Theorem parameter_tm_recursion0 =
+  parameter_gtm_recursion
+      |> INST_TYPE [alpha |-> rep_t, beta |-> unit_t, gamma |-> “:'r”]
+      |> Q.INST [‘lf’ |-> ‘^tlf’, ‘vf’ |-> ‘^tvf’, ‘vp’ |-> ‘^vp’,
+                 ‘lp’ |-> ‘^lp’]
+      |> SIMP_RULE (srw_ss()) [sumTheory.FORALL_SUM, FORALL_AND_THM,
+                               GSYM RIGHT_FORALL_IMP_THM, IMP_CONJ_THM,
+                               GSYM RIGHT_EXISTS_AND_THM,
+                               GSYM LEFT_EXISTS_AND_THM,
+                               GSYM LEFT_FORALL_IMP_THM,
+                               LIST_REL_CONS1, genind_GVAR,
+                               genind_GLAM_eqn, sidecond_def,
+                               NEWFCB_def, relsupp_def,
+                               LENGTH_NIL_SYM, LENGTH1, LENGTH2]
+      |> ONCE_REWRITE_RULE [termP']
+      |> SIMP_RULE (srw_ss() ++ DNF_ss) [LENGTH1, LENGTH2, LENGTH_NIL]
+      |> CONV_RULE (DEPTH_CONV termP_removal0)
+      |> CONV_RULE (DEPTH_CONV termP_removal1)
+      |> CONV_RULE (DEPTH_CONV termP_removal2)
+      |> SIMP_RULE (srw_ss()) [GSYM supp_npm, SYM term_REP_npm,
+                               GSYM supp_tpm, SYM term_REP_tpm,
+                               GSYM supp_rpm, SYM term_REP_rpm]
+      |> UNDISCH
+      |> rpt_hyp_dest_conj
+(*
+      |> lift_exfunction {repabs_pseudo_id = repabs_pseudo_id2,
+                          term_REP_t = term_REP_t2,
+                          cons_info = rcons_info}
+      |> lift_exfunction {repabs_pseudo_id = repabs_pseudo_id1,
+                          term_REP_t = term_REP_t1,
+                          cons_info = cons_info}
+      |> lift_exfunction {repabs_pseudo_id = repabs_pseudo_id0,
+                          term_REP_t = term_REP_t0,
+                          cons_info = ncons_info}
+      |> DISCH_ALL
+      |> elim_unnecessary_atoms {finite_fv = FINITE_FV}
+                                [ASSUME ``FINITE (A:string set)``,
+                                 ASSUME ``!p :'q. FINITE (supp ppm p)``]
+      |> UNDISCH_ALL |> DISCH_ALL
+      |> REWRITE_RULE [AND_IMP_INTRO]
+      |> CONV_RULE (LAND_CONV (REWRITE_CONV [GSYM CONJ_ASSOC]))
+      |> Q.INST [‘tvf’ |-> ‘vr’, (* Name? *)
+                 ‘tnf’ |-> ‘f0’, (* Nil *)
+                 ‘ttf’ |-> ‘f1’, (* Tau *)
+                 ‘tif’ |-> ‘f2’, (* Input *)
+                 ‘tof’ |-> ‘f3’, (* Output *)
+                 ‘tmf’ |-> ‘f4’, (* Match *)
+                 ‘tuf’ |-> ‘f5’, (* Mismatch *)
+                 ‘tsf’ |-> ‘f6’, (* Sum *)
+                 ‘tpf’ |-> ‘f7’, (* Par *)
+                 ‘trf’ |-> ‘f8’, (* Res *)
+                 ‘dpm’ |-> ‘apm’]
+      |> CONV_RULE (REDEPTH_CONV sort_uvars)
+
+Theorem tm_recursion =
+  parameter_tm_recursion
+      |> Q.INST_TYPE [‘:'q’ |-> ‘:unit’]
+      |> Q.INST [‘ppm’ |-> ‘discrete_pmact’,
+                  ‘vr’ |-> ‘\s u. vru s’,
+                  ‘pf’ |-> ‘\r a t u. pfu (r()) a t’,
+                  ‘sm’ |-> ‘\r1 r2 t1 t2 u. smu (r1()) (r2()) t1 t2’,
+                  ‘pr’ |-> ‘\r1 r2 t1 t2 u. pru (r1()) (r2()) t1 t2’,
+                  ‘rs’ |-> ‘\r L t u. rsu (r()) L t’,
+                  ‘rl’ |-> ‘\r t rf u. rlu (r()) t rf’,
+                  ‘re’ |-> ‘\r v t u. reu (r()) v t’]
+      |> SIMP_RULE (srw_ss()) [oneTheory.FORALL_ONE, oneTheory.FORALL_ONE_FN,
+                               oneTheory.EXISTS_ONE_FN, fnpm_def]
+      |> SIMP_RULE (srw_ss() ++ CONJ_ss) [supp_unitfn]
+      |> Q.INST [‘vru’ |-> ‘vr’,
+                 ‘pfu’ |-> ‘pf’,
+                 ‘smu’ |-> ‘sm’,
+                 ‘pru’ |-> ‘pr’,
+                 ‘rsu’ |-> ‘rs’,
+                 ‘rlu’ |-> ‘rl’,
+                 ‘reu’ |-> ‘re’]
+*)
 val _ = export_theory ();
 val _ = html_theory "pi_agent";
